theories/L/Complexity/Cook/Prelim.v
@@ -17,7 +17,20 @@ From Undecidability.L.TM Require Import TMflat TMflatEnc TMflatFun TMEncoding Ta
 
 Require Import Lia. 
 
+(*option monad in order to ease notation *)
+Definition optReturn := @Some.
+Definition optBind {X Y : Type} (x : option X) (f : X -> option Y) :=
+  match x with
+  | None => None
+  | Some x => f x
+  end. 
 
+(*notations from https://pdp7.org/blog/2011/01/the-maybe-monad-in-coq/ *)
+Notation "A >>= F" := (optBind A F) (at level 40, left associativity).
+Notation "'do' X <- A ; B" := (optBind A (fun X => B)) (at level 200, X ident, A at level 100, B at level 200).
+
+
+(* involutions *)
 Definition involution (X : Type) (f : X -> X) := forall (x : X), f (f x) = x. 
 
 Lemma map_involution (X : Type)(f : X -> X) : involution f -> involution (map f). 
