theories/L/Complexity/Reductions/kSAT_to_Clique.v
@@ -1,0 +1,308 @@
+From Undecidability.L Require Import L.
+From Undecidability.L.Tactics Require Import LTactics GenEncode.
+From Undecidability.L.Datatypes Require Import LLists LLNat LProd.
+From PslBase.FiniteTypes Require Import FinTypes Cardinality VectorFin.
+From Undecidability.L.Complexity.Problems Require Import newClique UGraph.
+From Undecidability.L.Complexity.Cook Require Import SAT kSAT Prelim.
+From Undecidability.L.Complexity.Reductions Require Pigeonhole.
+
+(** More preliminaries *)
+Section remove.
+  Variable (X : Type).
+  Context (eqdec : (forall x y: X, dec (x = y))).
+  Lemma in_remove_iff (l : list X) (a b : X) : a el remove eqdec b l <-> a el l /\ a <> b.
+  Proof.
+    revert a. induction l; intros; cbn.
+    - tauto. 
+    - destruct (eqdec b a).
+      + split; [firstorder | ].
+        intros [[-> | H1] H2]; [congruence|]. now apply IHl. 
+      + split; [firstorder; congruence | firstorder].
+  Qed. 
+
+  Lemma remove_length (l : list X) (a : X) : |remove eqdec a l| <= |l|.
+  Proof.
+    induction l; cbn.
+    - lia.
+    - destruct eqdec; cbn; lia. 
+  Qed. 
+
+  Lemma remove_length_el (l : list X) (a : X) : a el l -> |remove eqdec a l| < |l|.
+  Proof.
+    induction l.
+    - intros [].
+    - intros [-> | H1].
+      + cbn. destruct (eqdec a a); [specialize (remove_length l a); lia | congruence].
+      + cbn. destruct (eqdec a a0); [specialize (remove_length l a); lia | cbn; firstorder ].  
+  Qed. 
+End remove.
+
+
+Implicit Types (a : assgn) (N : cnf) (C : clause) (l :literal).
+
+Definition cnfGetClause N n := nth_error N n.
+Definition clauseGetLiteral C n := nth_error C n.
+Definition cnfGetLiteral N n1 n2 := 
+  do C <- cnfGetClause N n1;
+  clauseGetLiteral C n2.
+
+Section fixSAT.
+  Variable (k : nat). 
+  Variable (Hkgt : k > 0).
+  Variable (N : cnf).
+  Variable (Hkcnf : kCNF k N).
+
+  Definition Ncl := (|N|). 
+
+  Definition literalsConflict l1 l2 := 
+    let (b1, v1) := l1 in 
+    let (b2, v2) := l2 in 
+    v1 = v2 /\ b1 <> b2.
+
+  Definition opt_literalsConflict o1 o2 := 
+    match o1, o2 with 
+    | Some l1, Some l2 => literalsConflict l1 l2
+    | _, _ => False
+    end. 
+
+  (* the first component describes the literal, the second one the clause *)
+  Definition Vcnf := (Fin.t Ncl * Fin.t k)%type.
+  Implicit Type v : Vcnf. 
+
+  Definition Ecnf (p : Vcnf * Vcnf) := 
+    let (v1, v2) := p in 
+    let (ci1, li1) := v1 in 
+    let (ci2, li2) := v2 in
+    let o1 := cnfGetLiteral N (index ci1) (index li1) in
+    let o2 := cnfGetLiteral N (index ci2) (index li2) in 
+    not (opt_literalsConflict o1 o2) /\ ci1 <> ci2. 
+
+  Proposition literalsConflict_symm l1 l2 : literalsConflict l1 l2 <-> literalsConflict l2 l1. 
+  Proof. 
+    unfold literalsConflict. destruct l1, l2. split; intros [H1 H2]; split; congruence.
+  Qed.
+
+  Lemma Ecnf_symm v1 v2 : Ecnf (v1, v2) <-> Ecnf (v2, v1).
+  Proof. 
+    unfold Ecnf. destruct v1, v2. 
+    unfold opt_literalsConflict. destruct cnfGetLiteral, cnfGetLiteral.
+    2-4: firstorder. rewrite literalsConflict_symm. easy.
+  Qed. 
+
+  Lemma literalsConflict_dec l1 l2 : {literalsConflict l1 l2} + {~ literalsConflict l1 l2}.
+  Proof. 
+    unfold literalsConflict. 
+    destruct l1, l2. 
+    destruct (nat_eq_dec n n0).
+    - destruct (bool_eq_dec b b0); tauto.
+    - now right.
+  Defined. 
+
+  Lemma Ecnf_dec v1 v2 : {Ecnf (v1, v2) } + {not (Ecnf (v1, v2))}. 
+  Proof. 
+    unfold Ecnf. destruct v1 as (ci1 & li1), v2 as (ci2 & li2). 
+    unfold opt_literalsConflict.
+    destruct (eqType_dec ci1 ci2) as [He | He].
+    - destruct cnfGetLiteral; [ | now right].
+      destruct cnfGetLiteral; [ | now right].
+      destruct (literalsConflict_dec p p0); tauto. 
+    - destruct cnfGetLiteral; [ | now left].
+      destruct cnfGetLiteral; [ | now left].
+      destruct (literalsConflict_dec p p0); tauto.
+  Defined.
+
+  Definition Gcnf := Build_UGraph Ecnf_dec Ecnf_symm.
+
+  (** we show the correctness of the encoding *) 
+
+  Section SAT_implies_Clique.
+    (** Assume that there is a satisfying assignment for the CNF. *)
+    Variable (a__sat : assgn).
+    Context (H_sat : evalCnf a__sat N = true). 
+
+    Lemma evalLiteral_true_no_conflict a l1 l2 : evalLiteral a l1 = true -> evalLiteral a l2 = true -> not (literalsConflict l1 l2).
+    Proof using. 
+      clear k N a__sat Hkgt Hkcnf H_sat. 
+      intros H1 H2 H. unfold literalsConflict in H. 
+      destruct l1, l2. destruct H as [<- H]. 
+      unfold evalLiteral in *. 
+      rewrite Bool.eqb_true_iff in H1, H2. 
+      congruence.
+    Qed. 
+
+    Definition verticesClauseGe (L : list (V Gcnf)) (i : nat) := forall ci li, (ci, li) el L -> index ci >= i.
+
+    Definition literalInClause l C := l el C.
+    Definition literalInCnf l N := exists C, C el N /\ literalInClause l C. 
+
+    Proposition Vcnf_inhabitated : |N| > 0 -> exists (v : Vcnf), True.
+    Proof. 
+      clear H_sat.
+      Print Fin.t.
+      unfold Vcnf, Ncl.
+      intros H1. destruct k, N; cbn in *; try lia.
+      exists (@Fin.F1 (|l0|), @Fin.F1 n). easy.
+    Qed.
+
+    Lemma nth_index (t : finType) (def : t) i: i < (Cardinality t) -> index (nth i (elem t) def) = i.
+    Proof. 
+      intros H. 
+      unfold index. apply getPosition_nth. 
+      - apply Cardinality.dupfree_elements.
+      - apply H.
+    Qed.
+  
+    (*we fix the index of the clause: the same clause might appear twice, but for the proof, we really need to work on a particular clause given by an index *)
+    Lemma literalInClause_exists_vertex l C i: 
+      literalInClause l C -> cnfGetClause N i = Some C -> exists (v : V Gcnf), 
+      let (ci, li) := v in index ci = i /\ clauseGetLiteral C (index li) = Some l.
+    Proof.
+      clear H_sat.
+      intros H1 H2. 
+      destruct Vcnf_inhabitated as ((cdef & ldef) & _).
+      1: { unfold cnfGetClause in H2. apply nth_error_In in H2. destruct N; cbn in *; [destruct H2 | lia]. }
+      unfold literalInClause in H1. 
+      specialize (In_nth_error _ _ H1) as (j & H1').
+      unfold Gcnf, Vcnf. cbn [V]. 
+      exists (nth i (elem (finType_CS (Fin.t Ncl))) cdef, nth j (elem (finType_CS (Fin.t k))) ldef).
+      split. 
+      - apply nth_index. rewrite Card_Fint. unfold Ncl. eapply nth_error_Some_lt, H2. 
+      - unfold clauseGetLiteral. rewrite nth_index; [apply H1' | ]. 
+        rewrite Card_Fint. apply nth_error_Some_lt in H1'. 
+        rewrite kCNF_clause_length in Hkcnf.
+        unfold cnfGetClause in H2. apply nth_error_In in H2. 
+        apply Hkcnf in H2. lia.
+    Qed.
+      
+    Definition vertexSatisfied a (v : V (Gcnf)) := let (ci, li) := v in 
+      match cnfGetLiteral N (index ci) (index li) with 
+      | Some l => evalLiteral a__sat l = true
+      | None => False
+      end.  
+
+    Lemma vertexSatisfied_edge a ci ci' li li' : ci <> ci' -> vertexSatisfied a (ci, li) -> vertexSatisfied a (ci', li') -> E (((ci, li), (ci', li')) : (V Gcnf * V Gcnf)).
+    Proof. 
+      intros H. unfold vertexSatisfied.
+      unfold E. cbn. 
+      destruct cnfGetLiteral, cnfGetLiteral; try tauto.
+      intros H1 H2. unfold opt_literalsConflict. split; [now eapply evalLiteral_true_no_conflict | apply H].
+    Qed. 
+
+    Hint Constructors dupfree.
+    Lemma exists_clique' N' i : (exists N'', N = N'' ++ N') -> |N'| + i = |N| -> 
+        exists L, isKClique (|N'|) L /\ verticesClauseGe L i /\ (forall v, v el L -> vertexSatisfied a__sat v).
+    Proof. 
+      revert i. induction N'; cbn; intros. 
+      - exists []. unfold isKClique, verticesClauseGe. cbn. split; [split; [lia | ] | split; [intros ? _ [] | tauto]].
+        unfold isClique. split; [ intros ? ? [] | eauto].
+      - rename a into C. destruct H as (N'' & H). 
+        edestruct (IHN' (S i)) as (L & IH1 & IH2 & IH3).
+        2: lia.
+        1: { exists (N'' ++ [C]). rewrite H. rewrite <- app_assoc. now cbn. }
+        clear IHN'. 
+        rewrite H in H_sat. apply evalCnf_app_iff in H_sat as (_ & H_sat).
+        apply evalCnf_step_inv in H_sat as (b1 & b2 & H1 & H2 & H3).
+        symmetry in H3; apply andb_true_iff in H3 as [-> ->].
+        apply evalClause_literal_iff in H2 as (l & Hel & H2). 
+        edestruct (@literalInClause_exists_vertex l C (|N''|)) as (v & Hv). 
+        + unfold literalInClause. apply Hel.
+        + rewrite H. unfold cnfGetClause. rewrite nth_error_app2; [ | lia]. 
+          rewrite Nat.sub_diag. cbn. easy. 
+        + exists (v :: L). destruct v as (ci & li). destruct Hv as [Hv1 Hv2].
+          assert (vertexSatisfied a__sat (ci, li)) as H_sat.
+          { unfold vertexSatisfied. unfold cnfGetLiteral. 
+            rewrite Hv1, H. unfold cnfGetClause. rewrite nth_error_app2 by lia. rewrite Nat.sub_diag. 
+            cbn -[clauseGetLiteral index]. rewrite Hv2. apply H2.
+          } 
+          split; [ | split].
+          * apply indKClique_iff. constructor. 
+            -- apply indKClique_iff, IH1.  
+            -- unfold verticesClauseGe in IH2. intros H3%IH2. rewrite H, app_length in H0. cbn in H0. lia. 
+            -- intros (ci' & li') Hv'. specialize (IH3 _ Hv'). apply IH2 in Hv'. 
+               eapply vertexSatisfied_edge; [ rewrite H, app_length in H0; cbn in H0; intros ->; lia | apply H_sat | apply IH3]. 
+          * unfold verticesClauseGe. intros ci' li' [[=] | HL]; [ | specialize (IH2 _ _ HL); lia].
+            subst ci'. subst li'. rewrite Hv1. rewrite H, app_length in H0. cbn in H0. lia.
+          * intros v [<- | Hsat]; [ apply H_sat | now apply IH3].
+    Qed.
+
+    Lemma exists_clique: exists (L : list (V Gcnf)), isKClique Ncl L.
+    Proof. 
+      specialize (@exists_clique' N 0 ltac:(exists []; firstorder) ltac:(lia)) as (L & H & _). 
+      unfold Ncl. exists L; apply H.
+    Qed.
+  End SAT_implies_Clique. 
+
+  Section Clique_implies_SAT.
+    (** Assume that the graph has a clique *)
+    Variable (L : list (V Gcnf)). 
+    Context (Hclique : isKClique Ncl L). 
+    
+    (** The proof proceeds in three parts:
+        - We show that there exists a vertex of the clique for every clause of the CNF, using the pigeonhole principle.
+        - Thus, there exists a list of literals (one for every clause) which is non-contradictory.
+        - From this list of literals, a satisfying assignment can be derived. 
+      *)
+
+    (** * Step 1*)
+
+    (** proof by contradiction for decidable predicates *)
+    Fact contradiction_dec_bipredicate (X Y : Type) (p : X -> Y -> Prop) : (forall x y, dec (p x y)) -> forall x y, (~ (~ p x y)) -> p x y. 
+    Proof. 
+      intros Hdec x y Hdn. destruct (Hdec x y); tauto.
+    Qed.
+
+    Definition clausesOf (L : list (V Gcnf)) := map (fun '(ci, li) => ci) L. 
+    Lemma isClique_clausesOf_dupfree cl : isClique cl -> dupfree (clausesOf cl).
+    Proof. 
+      intros [H1 H2]. induction cl; cbn; [constructor | ].
+      destruct a as (ci & li). constructor.
+      - rewrite in_map_iff. intros ((ci' & li') & -> & H3).
+        destruct (eqType_dec li li') as [He | He]. 
+        + subst. inv H2. auto.
+        + specialize (H1 (ci, li) (ci, li') ltac:(now left) ltac:(now right) ltac:(congruence)). 
+          unfold E in H1. cbn in H1. destruct H1 as (_ & H1). congruence.
+      - apply IHcl; [ | now inv H2]. intros; now apply H1. 
+    Qed. 
+
+    Fact lt_le_rew (a b c : nat) : a < b -> b <= c -> a < c. 
+    Proof. lia. Qed.
+
+    Definition ofClause (v : V Gcnf) i := match v with (ci, li) => index ci = i end.  
+    Lemma clique_vertex_for_all_clauses : forall i, i < Ncl -> exists v, v el L /\ ofClause v i.
+    Proof. 
+      intros i Hi. eapply contradiction_dec_bipredicate with (p := fun i L => exists v : Vcnf, v el L /\ ofClause v i).
+      1: { clear i L Hclique Hi. intros i L. 
+           induction L. 
+           - right. intros (v & [] & _).
+           - destruct IHl as [IH | IH].
+             + left. destruct IH as (v & H1 & H2). now exists v.  
+             + destruct a as (ci & li). unfold ofClause. 
+               destruct (nat_eq_dec (index ci) i) as [H1 | H1]. 
+               * left. exists (ci, li). eauto.
+               * right. intros (v & [<- | H2] & H3); [congruence | apply IH; eauto].
+      } 
+      intros H. assert (forall v, v el L -> not (ofClause v i)) as H0.
+      { intros v Hel Hc. apply H; eauto. } 
+      clear H. 
+      enough (Pigeonhole.rep (clausesOf L)) as H. 
+      { apply Pigeonhole.not_dupfree_rep in H; [ | easy]. 
+        destruct Hclique as (_ & H1). now apply isClique_clausesOf_dupfree in H1. 
+      }
+      eapply Pigeonhole.pigeonhole; [easy | | ].
+      - instantiate (1 := remove (@eqType_dec (EqType (Fin.t Ncl))) (nth i (elem (finType_CS (Fin.t Ncl))) (Fin.of_nat_lt Hi)) (elem (finType_CS (Fin.t Ncl)))). 
+        intros ci Hel. apply in_remove_iff.
+        split; [apply elem_spec | ].
+        unfold clausesOf in Hel. apply in_map_iff in Hel as ((ci' & li) & -> & Hel).
+        apply H0 in Hel. unfold ofClause in Hel.
+        specialize (H0 (ci, Fin.of_nat_lt Hkgt)). intros Heq; apply Hel.
+        rewrite Heq. rewrite nth_index; [easy | rewrite Card_Fint; apply Hi].  
+      - unfold clausesOf. eapply lt_le_rew. 
+        + apply remove_length_el. apply elem_spec. 
+        + rewrite map_length. destruct Hclique as (H1 & _).
+          setoid_rewrite H1.
+          specialize (Card_Fint Ncl). unfold Cardinality. intros Heq. setoid_rewrite Heq. lia.
+    Qed.
+
+
+    (** Step 2 *)
+
